src/spec/TLS13.ConnectionState.ProtectedWireSegmentation.fsti
@@ -145,6 +145,47 @@ let paired_replay_split_prefixes_equal
     Seq.equal server_prefix_sent client_prefix_received /\
     Seq.equal client_prefix_sent server_prefix_received
 
+val lemma_same_endpoint_replay_split_prefixes_equal_empty
+  (model:CS.connection_model)
+  (suffix:list CS.conn_event)
+  (raw_sent:B.bytes)
+  (raw_received:B.bytes)
+  (final_model:CS.connection_model)
+  : Lemma
+      (same_endpoint_replay_split_prefixes_equal
+        model
+        []
+        suffix
+        raw_sent
+        raw_received
+        final_model)
+
+val lemma_paired_replay_split_prefixes_equal_empty
+  (server_model:CS.connection_model)
+  (client_model:CS.connection_model)
+  (server_suffix:list CS.conn_event)
+  (client_suffix:list CS.conn_event)
+  (server_full_sent:B.bytes)
+  (server_full_received:B.bytes)
+  (client_full_sent:B.bytes)
+  (client_full_received:B.bytes)
+  (server_final:CS.connection_model)
+  (client_final:CS.connection_model)
+  : Lemma
+      (paired_replay_split_prefixes_equal
+        server_model
+        client_model
+        []
+        server_suffix
+        []
+        client_suffix
+        server_full_sent
+        server_full_received
+        client_full_sent
+        client_full_received
+        server_final
+        client_final)
+
 val lemma_paired_replay_suffix_views_from_full_replays_with_equal_prefixes
   (server_model:CS.connection_model)
   (client_model:CS.connection_model)
